handling initial play requests that are malformed

src/Main.dfy
@@ -10,6 +10,7 @@ module CS886
   import opened Common.Data.String
   import opened Common.Data.Maybe
   import opened Common.Data.Result
+  import opened Common.Data.Seq
   import opened Commands
   import opened ConsoleIO
 
@@ -25,7 +26,7 @@ module CS886
   method REPL(prompt : string)
     decreases *
   {
-
+    var inGame := false;
     while true
       decreases *
     {
@@ -41,13 +42,28 @@ module CS886
         match cmd
         {
           case Help => runHelp();
-          case Quit => break;
-          case Play => print Play;
+          case Quit => {
+            if !inGame {
+              WriteLine("Exiting game.");
+              break;
+            } else {
+              WriteLine("Abaooning game, goodbye.");
+              break;
+            }
+          }
+          case Play(turns,sequence) => {
+            if inGame {
+              WriteLine("Cannot start a new game while in game.");
+            } else {
+              inGame := true;
+              WriteLine("Starting game.");
+              startGameProcess(turns,sequence,false);
+            }
+          }
         }
       }
     }
   }
-
 
   method runHelp()
   {
@@ -56,5 +72,55 @@ module CS886
     WriteLine(":play [n] [s] -- Play a game with 'n' tries and a secret sequence 's'");
     WriteLine(":guess [seq]  -- guess the secret");
     WriteLine(":stop         -- end game");
+  }
+
+  method startGameProcess(turns:Maybe<nat>, sequence: Maybe<seq<nat>>,inGame: bool)
+  requires !inGame
+  {
+    if isNothing(turns) || isNothing(sequence) {
+      WriteLine("Invalid command.");
+    }
+    var extractedTurns := extractTurns(turns);
+    var extractedSequence := extractSequence(sequence);
+    if (extractedTurns < 4) {
+      WriteLine("There should be at least 4 turns.");
+    }
+    if (CountElements(extractedSequence) < 4) {
+      WriteLine("The secret is too short.");
+    }
+
+  }
+
+
+  // Helpers
+
+  predicate isNothing<T>(m: Maybe<T>) {
+  match m {
+    case Nothing => true
+    case Just(_) => false
+    }
+  }
+  //@TODO: Need to add precondition that sequence is Just.
+  method extractSequence(m : Maybe<seq<nat>>)
+  returns (ret:seq<nat>)
+  {
+    match m {
+      case Just(value) => ret := value;
+      case Nothing => ret := [];
+    }
+  }
+  //TODO: Need to add precondition that turns is Just.
+  method extractTurns(m : Maybe<nat>)
+  returns (ret:nat)
+  {
+    match m {
+      case Just(value) => ret := value;
+      case Nothing => ret := 0;
+    }
+  }
+
+  function CountElements<T>(sequence: seq<T>): nat
+  {
+    |sequence|
   }
 }
